---
title: "ECON 110A notes"
author: "Haojie Liu"
date: "2023-06-02"
output: pdf_document
---

## Two-Period Neoclassical Consumption Model

### 1. The economy consists of a representative consumer who only lives for two periods: today (period 1), and the future (period 2).

### 2. The consumer earns income in both periods; can save (or borrow) and receives (or pays) some interest.

$Y_1$: income in period 1\newline
$Y_2$: income in period 2\newline
$S$: savings(borrowing)\newline\newline
$C_1$: consumptions in period 1\newline
$C_2$: consumptions in period 2\newline
$1+R$: gross interest rate\newline
$$Y_1 = C_1 + S$$
$$Y_2+S(1+R)=C_2$$ so $$Y_1=C_1+\frac{C_2-Y_2}{1+R}$$
$$C_1+\frac{C_2}{1+R}=Y_1+\frac{Y_2}{1+R}$$
$\frac{1}{1+R}$: price of consumption in the future in terms of consumption today\newline
$1+R$: Price of consumption today in terms of consumption in the future\newline


$$U(C_1)+\beta U(C_2), \space\space \beta\in[0,1]$$
$\triangle_1$: ice cream now\newline
$\beta\triangle_1$: ice cream future\newline


### 3. The consumer maximizes lifetime utility subject to the intertemporal budget constraint

$$max_{C_1,C_2} U(C_1)+\beta U(C_2)\space\space\space such\space that \space C_1+\frac{C_2}{1+R}=Y_1+\frac{Y_2}{1+R}$$
recall that $$S=Y_1-C_1$$

$$solution: U'(C_1)=\beta(1+R)U'(C_2)$$
$$U'(C)=\frac{dU(C)}{d(C)}$$

### Suppose: 

$$U'(C_1)>\beta(1+R)U'(C_2)$$

$$U'(C_1)<\beta(1+R)U'(C_2)$$

\newpage

## Gross Domestic Product

### Market value of the final goods and services produced in an economy over a certain period of time.

1. Market value – allows to add things up

2. Final – avoids double counting

3. Goods and Services – tangibles and intangibles

4. Produced – not all sales are GDP: used cars/houses, assets...

5. In an Economy – within certain boundaries (physical, political)

6. Certain Period of Time – GDP is a flow, not a stock


**Production = Income = Expenditure**


Production: value added produced\newline\newline
Income: remuneration to factors of production\newline\newline
Expenditure: end‐use of value added produced\newline\newline


### GDP by Value Added (= Sales – Cost of Inputs)

### GDP by Income (= Wages + Profits)

### The Expenditure Approach

$$GDP = C + I + G + X - IM$$

C: Private Consumption Expenditure\newline\newline
I: Private Investment Expenditure\newline\newline
G: Government Expenditure\newline\newline
X: Exports (Foreign Expenditure in Domestic Goods/Services)\newline\newline
IM: Imports (Domestic Expenditure in Foreign Goods/Services)\newline\newline


### GDP by Income (= Wages + Profits) = Wages and Benefits to Employees + Taxes (less subsidies) on Businesses + Profits + Depreciation of Fixed Capital

+ Wages: remuneration to labor as factor of production
+ Taxes: remuneration to government as factor of production
+ Profits: remuneration to owners/managers as factor of production
+ Depreciation of Fixed Capital: remuneration to capital as factor of production

## Nominal and Real GDP

$$GDP_t=\Sigma P^i_y \times Q^i_t$$
where i = food, rent, cars; t = time

$$RGDP_t=\Sigma P^i_X \times Q^i_t$$


+ Initial Price method(Laspeyres):$P^i_X$ areearliestdateprices
+ Final Price method (Paasche): $P^i_X$ are latest date prices
+ Chained‐Weighted method: $P^i_X$ are “weighted” averages across dates 


## The Role of Prices: Comparing GDP Across Countries

$$GDP^{CH}_{t,P^{US}}=GDP^{CH}_t \times E_t \times \frac{P_t^{US}}{P_t^{CH}}$$


$E_t$ (\$/¥): Exchange Rate(Dollars per Yuan)\newline\newline
$\frac{P_t^{US}}{P_t^{CH}}$: Price Level Ratio GDP Conversion Factor (World Bank Data)\newline\newline

## Growth Rate and Compounding

Growth rate $g$ of variable $y$ between $t$ and $t+1$

$$g_{t+1}=\frac{y_{t+1}-y_t}{y_t}$$
In percentage: $100\times g$


### Annualized growth rate $\bar g$ of variable y between year 0 and t assuming that previous growth is “reinvested”.

$$y_t= (1+\bar g)^ty_0$$


## GDP per Capita

$$y=\frac{Y}{L},k=\frac{K}{L}$$
$$y^*=\frac{Y^*}{L^*}=\frac{\bar A\bar K^{\alpha}\bar L^{1-\alpha}}{\bar L}=\bar A(\frac{\bar K}{\bar L})^\alpha$$
$$K^* = \frac{K^*}{L^*}=\frac{\bar K}{\bar L}$$
So $$y^*=\bar A(k^*)^\alpha$$




\newpage

# Production Model

## The Production Function

$$Y=F(A,K,L)$$

### Cobb-Douglas:

$$Y=AK^\alpha L^{1-\alpha}$$

+ F = production function
+ A = Ideas
+ K = capital
+ L = labor
+ Y = output "value added"


**Marginal Product**: extra output produced by increasing one factor while keeping all the other factors fixed.\newline\newline

**Diminishing Marginal Product**: Extra output produced by increasing one factor while keeping all the other fixed is decreasing in the one increasing factor.\newline\newline

$$MPL=\frac{dF(K,L)}{dL}$$
$$MPK=\frac{dF(K,L)}{dK}$$

+ Production Function: $F(K,L)=\bar A K^{\alpha}L^{1-\alpha}$
+ $MPL = (1-\alpha)\bar A K^{\alpha}L^{-\alpha}=(1-\alpha)\bar A(\frac{K}{L})^\alpha$
+ $MPK = \alpha\bar AK^{\alpha-1}L^{1-\alpha}=\alpha\bar A(\frac{L}{K})^{1-\alpha}$

**Returns to Scale (RS)**: change in output when all factors are changed by the same proportion.\newline\newline

$$F(\lambda K, \lambda L)=\lambda^sY, \lambda >0$$

+ S=1: constant return to scale
+ s>1: increasing returns to scale, $\lambda = 1.1$, $\lambda^2=1.1^2>1.1$
+ s<1: decreasing returns to scale, $\lambda = 1.1$, $\lambda^{\frac{1}{2}}=1.1^{\frac{1}{2}}<1.1$

**Assumption: Constant Returns to Scale (CRS)**: When all the production factors are scaled by $\lambda$, output is also scaled by $\lambda$.\newline\newline


## Profit Maximization

**Assumption**: Firms choose K and L such that profits are maximized.\newline\newline

$$\pi = P\times F(K,L)-r\times K-w\times L$$

+ w: wage rate
+ r: rental rate of capital
+ P: price of a unit of output = 1

*First order conditions*\newline\newline

$$K:\frac{d\pi}{dK}=0 \to \frac{dF(K,L)}{dK}-r=0$$
$$K:\frac{d\pi}{dL}=0 \to \frac{dF(K,L)}{dL}-w=0$$

so $MPL=w$, $MPK=r$\newline\newline


### Aggregation

**Assumption**: the total value added in the economy can be represented by the production function of a single “representative” firm where K is aggregate capital used in the economy, and L is total labor employed.

$$Y_A=F(K_A,L_A), Y_B=F(K_B,L_B)$$
$$Y=P_AY_A+P_BY_B$$
Aggregation: 

$$Y=F(K,L)$$

where: 
$$L=L_A+L_B,K=P^K_AK_A+P^K_BK_B$$

## Equilibrium

$$L^d=L^s, K^d=K^s$$
**unknowns: Y, K, L, w, r **
$$Y=\bar A K^{\alpha}L^{1-\alpha}$$
$$r=\alpha\bar A(\frac{L}{K})^{1-\alpha}(=MPK)$$
$$w=(1-\alpha)\bar A(\frac{K}{L})^{\alpha}(=MPL)$$
$$L=\bar L, K=\bar K$$

**solution:$Y^*,K^*,L^*,W^*,r^*$**



$$L^*=\bar L, K^*=\bar K$$
$$Y=\bar A K^{\alpha}L^{1-\alpha}$$

$$r^*=\alpha\bar A(\frac{\bar L}{K})^{1-\alpha}$$

$$w^*=(1-\alpha)\bar A(\frac{\bar K}{L})^{\alpha}$$


$$Y^*=\bar A\bar K^{\alpha}\bar L^{1-\alpha}$$

### Production Model: 4 Implications

1. All available factors are utilized in equilibrium, so production depends on endowments of factors


$$Y=\bar A\bar K^\alpha\bar L^{1-\alpha}$$


2. Total payments to factors as share of output (factor shares) are determined by the production function

Labor share: 
$$\frac{w^*\times L^*}{Y^*}=\frac{(1-\alpha)\bar A(\frac{\bar K}{\bar L})^\alpha \times \bar L}{\bar A \bar K^{\alpha}\bar L^{1-\alpha}}=1-\alpha$$
Capital share: 
$$\frac{w^*\times L^*}{Y^*}=\frac{\alpha\bar A(\frac{\bar L}{\bar K})^{1-\alpha}}{\bar A \bar K^{\alpha}\bar L^{1-\alpha}}=\alpha$$

3. Production (value added) is equal to Income

$$Y^*=\bar K^\alpha\bar L^{1-\alpha}=r^*\times K^*+w^*\times L^*$$
4. The profits of the representative firm are zero

$$\pi^* = Y^*-r^*\times K^*-w^*\times L^*=0$$

\newpage 

# Solow Model

### Production

$$Y_t=\bar AK_t^\alpha L_t^{1-\alpha}, t\in[1,\inf]$$

### Resource Constraint

$$Y_t=C_t+S_t$$

### Capital Accumulation


$$K_{t+1}=K_t+I_t-\bar dK_t$$
define $$\triangle K_{t+1}=K_{t+1}-K_t$$
then $$\triangle K_{t+1}=I_t-\bar dK_t$$

$\bar d$: depreciation rate\newline\newline
$I_t$: Investment


### Labor

$$L_t=\bar L$$


### Investment

$$I_t=S_t$$
$$S_t=\bar sY_t$$

$\bar s$: saving rate (investment rate)\newline\newline




### Solve Equations

Start $$I^t=\bar sY_t$$ and sub into $\triangle K_{t+1}$: $$\triangle K_{t+1}=\bar sY_t-\bar dK_t$$ note $$Y_t=\bar AK_t^\alpha L_t^{1-\alpha}-dK_t$$



![](/Users/liuhaojie/Desktop/UCSDECON110A/p1.jpg){width=70%}

![](/Users/liuhaojie/Desktop/UCSDECON110A/p2.jpg){width=70%}


### Long Run: Steady State Capital

$$K^*:\triangle K_{t+1}=0 \to \bar s \bar A K^{*\alpha}\bar L^{1-\alpha}=\bar dK^*$$
solve for $K^*:$

$$\frac{\bar s}{\bar d}\bar A\bar L^{1-\alpha}=\frac{K^*}{K^{*\alpha}}=K^{*1-\alpha}$$
$$(K^{*1-\alpha})^{\frac{1}{1-\alpha}}=(\frac{\bar s}{\bar d}\bar A \bar L^{1-\alpha})^{\frac{1}{1-\alpha}}\to K^*=(\frac{\bar s}{\bar d}\bar A)^{\frac{1}{1-\alpha}}\bar L$$
capital per-worker in steady state:

$$\frac{K^*}{\bar L} = (\frac{\bar s}{\bar d}\bar A)^{\frac{1}{1-\alpha}}$$

$$Y^*=\bar AK^{*\alpha}\bar L^{1-\alpha}$$
$$=\bar A[(\frac{\bar s}{\bar d}\bar A)^{\frac{1}{1-\alpha}}\bar L]^\alpha\bar L^{1-\alpha}$$
$$=\bar A ^{1+\frac{\alpha}{1+\alpha}}(\frac{\bar s}{\bar d})^{\frac{\alpha}{1-\alpha}}\bar L$$
$$\bar A ^{\frac{1}{1-\alpha}}(\frac{\bar s}{\bar d})^{\frac{\alpha}{1-\alpha}}\bar L$$

$$y^*=\frac{Y^*}{\bar L}=\bar A^{\frac{1}{1-\alpha}}(\frac{\bar s}{\bar d})^{\frac{\alpha}{1-\alpha}}$$
set $\alpha=\frac{1}{3}$

$$y^*=\bar A^{\frac{3}{2}}(\frac{\bar s}{\bar d})^\frac{1}{2}$$

![](/Users/liuhaojie/Desktop/UCSDECON110A/p3.png){width=70%}

![](/Users/liuhaojie/Desktop/UCSDECON110A/p5.png){width=70%}

![](/Users/liuhaojie/Desktop/UCSDECON110A/p6.png){width=70%}

### The Real Interest Rate

Amount of output a person can earn by saving one unit of output for a year, or amount of output a person must pay to borrow one unit of output for a year.


![](/Users/liuhaojie/Desktop/UCSDECON110A/p7.png){width=70%}




![](/Users/liuhaojie/Desktop/UCSDECON110A/p8.png){width=70%}


![](/Users/liuhaojie/Desktop/UCSDECON110A/p9.png){width=70%}

### Experiment 3: Increase in Population, $\bar L$

### What is the effect :on output per worker (GDP per capita)?

$$Y^* = \bar A^{\frac{1}{1-\alpha}}(\frac{\bar s}{\bar d})^{\frac{\alpha}{1-\alpha}}$$
No impact in steady state

$$Y^N_0=\frac{\bar A K^{*\alpha}\bar L_N^{1-\alpha}}{\bar L_N}=\bar A(\frac{K^*}{\bar L_N})<\bar A(\frac{K^*}{\bar L})^\alpha=Y^*$$



![](/Users/liuhaojie/Desktop/UCSDECON110A/p10.png){width=70%}


![](/Users/liuhaojie/Desktop/UCSDECON110A/p11.png){width=70%}


![](/Users/liuhaojie/Desktop/UCSDECON110A/p12.png){width=70%}



### The Principle of Transition Dynamics

The farther below the steady state capital an economy is, the faster the economy will grow.


![](/Users/liuhaojie/Desktop/UCSDECON110A/p13.png){width=70%}


$$\frac{\triangle K_{t+1}}{K_t}=\bar s\frac{Y^*}{K^*}((\frac{K^*}{K_t})^{1-\alpha}-1)$$

$$Y=\bar A K^\alpha \bar L^{1-\alpha}$$
$$ln(Y_t)=ln(\bar A)+\alpha ln(K)+(1-\alpha)ln(\bar L)$$
$$g_Y=\frac{\triangle Y_t}{Y_t}=\alpha\frac{\triangle K_t}{K_t}=g_K$$

### No-Arbitrage Equation for Investment


Consider a firm thinking of investing  $\$P_K$ . The firm has two options: bank deposit or physical capital\newline


\begin{center}Bank Deposit \space \space \space \space \space"No-Arbitrage"\space \space Physical Capital(rent out)\end{center}
$$\frac{P_K(1+R)}{P_K}-\frac{P_K}{P_K} \ \ \ \ \ \ \ \ =\ \ \ \ \ \ \ \frac{r\times P_K+P_K^{used}}{P_K}-\frac{P_K}{P_K}$$

$$R=r+\frac{P^u_K-P_K}{P_K}\to \frac{P'_K-P_K}{P_K}-d \to \frac{\triangle P_K}{P_K}-\bar d$$
$$R=r+\frac{\triangle P_K}{P_K}-\bar d$$

### The User Cost of Capital

$$MPK = R+\bar d-\frac{\triangle P_K}{P_K}=uc$$

+ R: opportunity cost of funds
+ $\bar d$: depreciation cost
+ $\frac{\triangle P_K}{P_K}$: capital gain (if +)/ loss (if -)


### Ideas are Nonrivalrous

Important: distinguish nonrivalry from scarcity and excludability

+ nonrivalry: once they are created, it is feasible for ideas to be used by anybody 
+ scarcity: new ideas are scarce, always better to have more
+ excludability: use of ideas can be restricted by property rights


### Production and Cost


+ Production: $Y=L^\alpha$
+ Fixed Cost: $F$
+ Total Function: $C=F+w\times L, L=Y^{\frac{1}{2}}$
+ Cost Function : $C(Y)=F+w\times Y^{\frac{1}{2}}$
+ Marginal Cost: $MC=\frac{dC(Y)}{dY}=\frac{1}{2}+w\times Y^{\frac{1-\alpha}{\alpha}}$
+ Average Cost: $AC=\frac{C(Y)}{Y}=\frac{F}{Y}+\frac{wY^{\frac{1}{2}}}{Y}=\frac{F}{Y}+wY^{\frac{1-\alpha}{\alpha}}$
+ Profits per unit: $\frac{\pi}{Y}=\frac{P\times Y-C(Y)}{Y}=P-AC$

### Returns to Scale and Average Cost

Average Cost: $$AC(Y)=\frac{C(Y)}{Y}$$ $$AC(Y)increasing in Y: decreasing RS$$ $$AC(Y)constant in Y: constant RS$$ $$AC(Y)decreasing in Y: increasing RS$$


### Fixed Cost, Average Cost, and Increasing Returns to Scale

Production: $Y=L$\newline
Fixed Cost: F

+ $F=0, C(Y)=wY,AC(Y)=w$
+ $F>0$


$$Y$$ $$= 0 when C(Y)\le F \to AC(Y)=\frac{wL+F}{Y}=\frac{wY+F}{Y}=w+\frac{F}{Y}=\infty$$ $$= L when C(Y)>F\to AC(Y)=\frac{F}{Y}+\frac{wL}{Y}=\frac{F}{Y}+w$$

decreasing in Y, so increasing returns!
















